feat: Adding a storage option to the KeyStore
The key store now allows for both a default DynamoDB table,
or any custom storage system.

The important aspect about the key store
is the fact that branch keys can be versioned easily,
and are cryptographically safe to use.
The actual storage medium is not important.

See: https://github.com/awslabs/aws-encryption-sdk-specification/blob/master/changes/2024-6-17_key-store-persistance/background.md#background

AwsCryptographicMaterialProviders/runtimes/java/src/main/smithy-generated/software/amazon/cryptography/keystore/EncryptedKeyStore.java
@@ -1,0 +1,336 @@
+// Copyright Amazon.com Inc. or its affiliates. All Rights Reserved.
+// SPDX-License-Identifier: Apache-2.0
+// Do not modify this file. This file is machine generated, and any changes to it will be overwritten.
+package software.amazon.cryptography.keystore;
+
+import Wrappers_Compile.Result;
+import java.lang.IllegalArgumentException;
+import java.lang.RuntimeException;
+import java.util.Objects;
+import software.amazon.cryptography.keystore.internaldafny.types.Error;
+import software.amazon.cryptography.keystore.model.GetEncryptedActiveBranchKeyInput;
+import software.amazon.cryptography.keystore.model.GetEncryptedActiveBranchKeyOutput;
+import software.amazon.cryptography.keystore.model.GetEncryptedBeaconKeyInput;
+import software.amazon.cryptography.keystore.model.GetEncryptedBeaconKeyOutput;
+import software.amazon.cryptography.keystore.model.GetEncryptedBranchKeyVersionInput;
+import software.amazon.cryptography.keystore.model.GetEncryptedBranchKeyVersionOutput;
+import software.amazon.cryptography.keystore.model.GetTableNameInput;
+import software.amazon.cryptography.keystore.model.GetTableNameOutput;
+import software.amazon.cryptography.keystore.model.WriteNewBranchKeyVersionToKeystoreInput;
+import software.amazon.cryptography.keystore.model.WriteNewBranchKeyVersionToKeystoreOutput;
+import software.amazon.cryptography.keystore.model.WriteNewKeyToStoreInput;
+import software.amazon.cryptography.keystore.model.WriteNewKeyToStoreOutput;
+
+public final class EncryptedKeyStore implements IEncryptedKeyStore {
+
+  private final software.amazon.cryptography.keystore.internaldafny.types.IEncryptedKeyStore _impl;
+
+  private EncryptedKeyStore(
+    software.amazon.cryptography.keystore.internaldafny.types.IEncryptedKeyStore iEncryptedKeyStore
+  ) {
+    Objects.requireNonNull(
+      iEncryptedKeyStore,
+      "Missing value for required argument `iEncryptedKeyStore`"
+    );
+    this._impl = iEncryptedKeyStore;
+  }
+
+  public static EncryptedKeyStore wrap(
+    software.amazon.cryptography.keystore.internaldafny.types.IEncryptedKeyStore iEncryptedKeyStore
+  ) {
+    return new EncryptedKeyStore(iEncryptedKeyStore);
+  }
+
+  public static <I extends IEncryptedKeyStore> EncryptedKeyStore wrap(
+    I iEncryptedKeyStore
+  ) {
+    Objects.requireNonNull(
+      iEncryptedKeyStore,
+      "Missing value for required argument `iEncryptedKeyStore`"
+    );
+    if (
+      iEncryptedKeyStore instanceof
+      software.amazon.cryptography.keystore.EncryptedKeyStore
+    ) {
+      return ((EncryptedKeyStore) iEncryptedKeyStore);
+    }
+    return EncryptedKeyStore.wrap(new NativeWrapper(iEncryptedKeyStore));
+  }
+
+  public software.amazon.cryptography.keystore.internaldafny.types.IEncryptedKeyStore impl() {
+    return this._impl;
+  }
+
+  public GetEncryptedActiveBranchKeyOutput GetEncryptedActiveBranchKey(
+    GetEncryptedActiveBranchKeyInput input
+  ) {
+    software.amazon.cryptography.keystore.internaldafny.types.GetEncryptedActiveBranchKeyInput dafnyValue =
+      ToDafny.GetEncryptedActiveBranchKeyInput(input);
+    Result<
+      software.amazon.cryptography.keystore.internaldafny.types.GetEncryptedActiveBranchKeyOutput,
+      Error
+    > result = this._impl.GetEncryptedActiveBranchKey(dafnyValue);
+    if (result.is_Failure()) {
+      throw ToNative.Error(result.dtor_error());
+    }
+    return ToNative.GetEncryptedActiveBranchKeyOutput(result.dtor_value());
+  }
+
+  public GetEncryptedBeaconKeyOutput GetEncryptedBeaconKey(
+    GetEncryptedBeaconKeyInput input
+  ) {
+    software.amazon.cryptography.keystore.internaldafny.types.GetEncryptedBeaconKeyInput dafnyValue =
+      ToDafny.GetEncryptedBeaconKeyInput(input);
+    Result<
+      software.amazon.cryptography.keystore.internaldafny.types.GetEncryptedBeaconKeyOutput,
+      Error
+    > result = this._impl.GetEncryptedBeaconKey(dafnyValue);
+    if (result.is_Failure()) {
+      throw ToNative.Error(result.dtor_error());
+    }
+    return ToNative.GetEncryptedBeaconKeyOutput(result.dtor_value());
+  }
+
+  public GetEncryptedBranchKeyVersionOutput GetEncryptedBranchKeyVersion(
+    GetEncryptedBranchKeyVersionInput input
+  ) {
+    software.amazon.cryptography.keystore.internaldafny.types.GetEncryptedBranchKeyVersionInput dafnyValue =
+      ToDafny.GetEncryptedBranchKeyVersionInput(input);
+    Result<
+      software.amazon.cryptography.keystore.internaldafny.types.GetEncryptedBranchKeyVersionOutput,
+      Error
+    > result = this._impl.GetEncryptedBranchKeyVersion(dafnyValue);
+    if (result.is_Failure()) {
+      throw ToNative.Error(result.dtor_error());
+    }
+    return ToNative.GetEncryptedBranchKeyVersionOutput(result.dtor_value());
+  }
+
+  public GetTableNameOutput GetTableName(GetTableNameInput input) {
+    software.amazon.cryptography.keystore.internaldafny.types.GetTableNameInput dafnyValue =
+      ToDafny.GetTableNameInput(input);
+    Result<
+      software.amazon.cryptography.keystore.internaldafny.types.GetTableNameOutput,
+      Error
+    > result = this._impl.GetTableName(dafnyValue);
+    if (result.is_Failure()) {
+      throw ToNative.Error(result.dtor_error());
+    }
+    return ToNative.GetTableNameOutput(result.dtor_value());
+  }
+
+  public WriteNewBranchKeyVersionToKeystoreOutput WriteNewBranchKeyVersionToKeystore(
+    WriteNewBranchKeyVersionToKeystoreInput input
+  ) {
+    software.amazon.cryptography.keystore.internaldafny.types.WriteNewBranchKeyVersionToKeystoreInput dafnyValue =
+      ToDafny.WriteNewBranchKeyVersionToKeystoreInput(input);
+    Result<
+      software.amazon.cryptography.keystore.internaldafny.types.WriteNewBranchKeyVersionToKeystoreOutput,
+      Error
+    > result = this._impl.WriteNewBranchKeyVersionToKeystore(dafnyValue);
+    if (result.is_Failure()) {
+      throw ToNative.Error(result.dtor_error());
+    }
+    return ToNative.WriteNewBranchKeyVersionToKeystoreOutput(
+      result.dtor_value()
+    );
+  }
+
+  public WriteNewKeyToStoreOutput WriteNewKeyToStore(
+    WriteNewKeyToStoreInput input
+  ) {
+    software.amazon.cryptography.keystore.internaldafny.types.WriteNewKeyToStoreInput dafnyValue =
+      ToDafny.WriteNewKeyToStoreInput(input);
+    Result<
+      software.amazon.cryptography.keystore.internaldafny.types.WriteNewKeyToStoreOutput,
+      Error
+    > result = this._impl.WriteNewKeyToStore(dafnyValue);
+    if (result.is_Failure()) {
+      throw ToNative.Error(result.dtor_error());
+    }
+    return ToNative.WriteNewKeyToStoreOutput(result.dtor_value());
+  }
+
+  protected static final class NativeWrapper
+    implements
+      software.amazon.cryptography.keystore.internaldafny.types.IEncryptedKeyStore {
+
+    protected final IEncryptedKeyStore _impl;
+
+    NativeWrapper(IEncryptedKeyStore nativeImpl) {
+      if (nativeImpl instanceof EncryptedKeyStore) {
+        throw new IllegalArgumentException(
+          "Recursive wrapping is strictly forbidden."
+        );
+      }
+      this._impl = nativeImpl;
+    }
+
+    public Result<
+      software.amazon.cryptography.keystore.internaldafny.types.GetEncryptedActiveBranchKeyOutput,
+      Error
+    > GetEncryptedActiveBranchKey(
+      software.amazon.cryptography.keystore.internaldafny.types.GetEncryptedActiveBranchKeyInput dafnyInput
+    ) {
+      try {
+        GetEncryptedActiveBranchKeyInput nativeInput =
+          ToNative.GetEncryptedActiveBranchKeyInput(dafnyInput);
+        GetEncryptedActiveBranchKeyOutput nativeOutput =
+          this._impl.GetEncryptedActiveBranchKey(nativeInput);
+        software.amazon.cryptography.keystore.internaldafny.types.GetEncryptedActiveBranchKeyOutput dafnyOutput =
+          ToDafny.GetEncryptedActiveBranchKeyOutput(nativeOutput);
+        return Result.create_Success(dafnyOutput);
+      } catch (RuntimeException ex) {
+        return Result.create_Failure(ToDafny.Error(ex));
+      }
+    }
+
+    public Result<
+      software.amazon.cryptography.keystore.internaldafny.types.GetEncryptedActiveBranchKeyOutput,
+      Error
+    > GetEncryptedActiveBranchKey_k(
+      software.amazon.cryptography.keystore.internaldafny.types.GetEncryptedActiveBranchKeyInput dafnyInput
+    ) {
+      throw new RuntimeException("Not supported at this time.");
+    }
+
+    public Result<
+      software.amazon.cryptography.keystore.internaldafny.types.GetEncryptedBeaconKeyOutput,
+      Error
+    > GetEncryptedBeaconKey(
+      software.amazon.cryptography.keystore.internaldafny.types.GetEncryptedBeaconKeyInput dafnyInput
+    ) {
+      try {
+        GetEncryptedBeaconKeyInput nativeInput =
+          ToNative.GetEncryptedBeaconKeyInput(dafnyInput);
+        GetEncryptedBeaconKeyOutput nativeOutput =
+          this._impl.GetEncryptedBeaconKey(nativeInput);
+        software.amazon.cryptography.keystore.internaldafny.types.GetEncryptedBeaconKeyOutput dafnyOutput =
+          ToDafny.GetEncryptedBeaconKeyOutput(nativeOutput);
+        return Result.create_Success(dafnyOutput);
+      } catch (RuntimeException ex) {
+        return Result.create_Failure(ToDafny.Error(ex));
+      }
+    }
+
+    public Result<
+      software.amazon.cryptography.keystore.internaldafny.types.GetEncryptedBeaconKeyOutput,
+      Error
+    > GetEncryptedBeaconKey_k(
+      software.amazon.cryptography.keystore.internaldafny.types.GetEncryptedBeaconKeyInput dafnyInput
+    ) {
+      throw new RuntimeException("Not supported at this time.");
+    }
+
+    public Result<
+      software.amazon.cryptography.keystore.internaldafny.types.GetEncryptedBranchKeyVersionOutput,
+      Error
+    > GetEncryptedBranchKeyVersion(
+      software.amazon.cryptography.keystore.internaldafny.types.GetEncryptedBranchKeyVersionInput dafnyInput
+    ) {
+      try {
+        GetEncryptedBranchKeyVersionInput nativeInput =
+          ToNative.GetEncryptedBranchKeyVersionInput(dafnyInput);
+        GetEncryptedBranchKeyVersionOutput nativeOutput =
+          this._impl.GetEncryptedBranchKeyVersion(nativeInput);
+        software.amazon.cryptography.keystore.internaldafny.types.GetEncryptedBranchKeyVersionOutput dafnyOutput =
+          ToDafny.GetEncryptedBranchKeyVersionOutput(nativeOutput);
+        return Result.create_Success(dafnyOutput);
+      } catch (RuntimeException ex) {
+        return Result.create_Failure(ToDafny.Error(ex));
+      }
+    }
+
+    public Result<
+      software.amazon.cryptography.keystore.internaldafny.types.GetEncryptedBranchKeyVersionOutput,
+      Error
+    > GetEncryptedBranchKeyVersion_k(
+      software.amazon.cryptography.keystore.internaldafny.types.GetEncryptedBranchKeyVersionInput dafnyInput
+    ) {
+      throw new RuntimeException("Not supported at this time.");
+    }
+
+    public Result<
+      software.amazon.cryptography.keystore.internaldafny.types.GetTableNameOutput,
+      Error
+    > GetTableName(
+      software.amazon.cryptography.keystore.internaldafny.types.GetTableNameInput dafnyInput
+    ) {
+      try {
+        GetTableNameInput nativeInput = ToNative.GetTableNameInput(dafnyInput);
+        GetTableNameOutput nativeOutput = this._impl.GetTableName(nativeInput);
+        software.amazon.cryptography.keystore.internaldafny.types.GetTableNameOutput dafnyOutput =
+          ToDafny.GetTableNameOutput(nativeOutput);
+        return Result.create_Success(dafnyOutput);
+      } catch (RuntimeException ex) {
+        return Result.create_Failure(ToDafny.Error(ex));
+      }
+    }
+
+    public Result<
+      software.amazon.cryptography.keystore.internaldafny.types.GetTableNameOutput,
+      Error
+    > GetTableName_k(
+      software.amazon.cryptography.keystore.internaldafny.types.GetTableNameInput dafnyInput
+    ) {
+      throw new RuntimeException("Not supported at this time.");
+    }
+
+    public Result<
+      software.amazon.cryptography.keystore.internaldafny.types.WriteNewBranchKeyVersionToKeystoreOutput,
+      Error
+    > WriteNewBranchKeyVersionToKeystore(
+      software.amazon.cryptography.keystore.internaldafny.types.WriteNewBranchKeyVersionToKeystoreInput dafnyInput
+    ) {
+      try {
+        WriteNewBranchKeyVersionToKeystoreInput nativeInput =
+          ToNative.WriteNewBranchKeyVersionToKeystoreInput(dafnyInput);
+        WriteNewBranchKeyVersionToKeystoreOutput nativeOutput =
+          this._impl.WriteNewBranchKeyVersionToKeystore(nativeInput);
+        software.amazon.cryptography.keystore.internaldafny.types.WriteNewBranchKeyVersionToKeystoreOutput dafnyOutput =
+          ToDafny.WriteNewBranchKeyVersionToKeystoreOutput(nativeOutput);
+        return Result.create_Success(dafnyOutput);
+      } catch (RuntimeException ex) {
+        return Result.create_Failure(ToDafny.Error(ex));
+      }
+    }
+
+    public Result<
+      software.amazon.cryptography.keystore.internaldafny.types.WriteNewBranchKeyVersionToKeystoreOutput,
+      Error
+    > WriteNewBranchKeyVersionToKeystore_k(
+      software.amazon.cryptography.keystore.internaldafny.types.WriteNewBranchKeyVersionToKeystoreInput dafnyInput
+    ) {
+      throw new RuntimeException("Not supported at this time.");
+    }
+
+    public Result<
+      software.amazon.cryptography.keystore.internaldafny.types.WriteNewKeyToStoreOutput,
+      Error
+    > WriteNewKeyToStore(
+      software.amazon.cryptography.keystore.internaldafny.types.WriteNewKeyToStoreInput dafnyInput
+    ) {
+      try {
+        WriteNewKeyToStoreInput nativeInput = ToNative.WriteNewKeyToStoreInput(
+          dafnyInput
+        );
+        WriteNewKeyToStoreOutput nativeOutput =
+          this._impl.WriteNewKeyToStore(nativeInput);
+        software.amazon.cryptography.keystore.internaldafny.types.WriteNewKeyToStoreOutput dafnyOutput =
+          ToDafny.WriteNewKeyToStoreOutput(nativeOutput);
+        return Result.create_Success(dafnyOutput);
+      } catch (RuntimeException ex) {
+        return Result.create_Failure(ToDafny.Error(ex));
+      }
+    }
+
+    public Result<
+      software.amazon.cryptography.keystore.internaldafny.types.WriteNewKeyToStoreOutput,
+      Error
+    > WriteNewKeyToStore_k(
+      software.amazon.cryptography.keystore.internaldafny.types.WriteNewKeyToStoreInput dafnyInput
+    ) {
+      throw new RuntimeException("Not supported at this time.");
+    }
+  }
+}
