AwsCryptographicMaterialProviders/runtimes/java/src/main/smithy-generated/software/amazon/cryptography/keystore/IEncryptedKeyStore.java
@@ -1,0 +1,39 @@
+// Copyright Amazon.com Inc. or its affiliates. All Rights Reserved.
+// SPDX-License-Identifier: Apache-2.0
+// Do not modify this file. This file is machine generated, and any changes to it will be overwritten.
+package software.amazon.cryptography.keystore;
+
+import software.amazon.cryptography.keystore.model.GetEncryptedActiveBranchKeyInput;
+import software.amazon.cryptography.keystore.model.GetEncryptedActiveBranchKeyOutput;
+import software.amazon.cryptography.keystore.model.GetEncryptedBeaconKeyInput;
+import software.amazon.cryptography.keystore.model.GetEncryptedBeaconKeyOutput;
+import software.amazon.cryptography.keystore.model.GetEncryptedBranchKeyVersionInput;
+import software.amazon.cryptography.keystore.model.GetEncryptedBranchKeyVersionOutput;
+import software.amazon.cryptography.keystore.model.GetTableNameInput;
+import software.amazon.cryptography.keystore.model.GetTableNameOutput;
+import software.amazon.cryptography.keystore.model.WriteNewBranchKeyVersionToKeystoreInput;
+import software.amazon.cryptography.keystore.model.WriteNewBranchKeyVersionToKeystoreOutput;
+import software.amazon.cryptography.keystore.model.WriteNewKeyToStoreInput;
+import software.amazon.cryptography.keystore.model.WriteNewKeyToStoreOutput;
+
+public interface IEncryptedKeyStore {
+  GetEncryptedActiveBranchKeyOutput GetEncryptedActiveBranchKey(
+    GetEncryptedActiveBranchKeyInput input
+  );
+
+  GetEncryptedBeaconKeyOutput GetEncryptedBeaconKey(
+    GetEncryptedBeaconKeyInput input
+  );
+
+  GetEncryptedBranchKeyVersionOutput GetEncryptedBranchKeyVersion(
+    GetEncryptedBranchKeyVersionInput input
+  );
+
+  GetTableNameOutput GetTableName(GetTableNameInput input);
+
+  WriteNewBranchKeyVersionToKeystoreOutput WriteNewBranchKeyVersionToKeystore(
+    WriteNewBranchKeyVersionToKeystoreInput input
+  );
+
+  WriteNewKeyToStoreOutput WriteNewKeyToStore(WriteNewKeyToStoreInput input);
+}
