AwsCryptographicMaterialProviders/runtimes/java/src/main/smithy-generated/software/amazon/cryptography/keystore/ToNative.java
@@ -17,28 +17,47 @@ import software.amazon.cryptography.keystore.internaldafny.types.Error_Collectio
 import software.amazon.cryptography.keystore.internaldafny.types.Error_KeyStoreException;
 import software.amazon.cryptography.keystore.internaldafny.types.Error_Opaque;
 import software.amazon.cryptography.keystore.internaldafny.types.IKeyStoreClient;
+import software.amazon.cryptography.keystore.model.ActiveHierarchicalSymmetricBeacon;
+import software.amazon.cryptography.keystore.model.AwsKms;
 import software.amazon.cryptography.keystore.model.BeaconKeyMaterials;
 import software.amazon.cryptography.keystore.model.BranchKeyMaterials;
+import software.amazon.cryptography.keystore.model.BranchKeyType;
 import software.amazon.cryptography.keystore.model.CollectionOfErrors;
 import software.amazon.cryptography.keystore.model.CreateKeyInput;
 import software.amazon.cryptography.keystore.model.CreateKeyOutput;
 import software.amazon.cryptography.keystore.model.CreateKeyStoreInput;
 import software.amazon.cryptography.keystore.model.CreateKeyStoreOutput;
 import software.amazon.cryptography.keystore.model.Discovery;
+import software.amazon.cryptography.keystore.model.DynamoDBTable;
+import software.amazon.cryptography.keystore.model.EncryptedHierarchicalKey;
 import software.amazon.cryptography.keystore.model.GetActiveBranchKeyInput;
 import software.amazon.cryptography.keystore.model.GetActiveBranchKeyOutput;
 import software.amazon.cryptography.keystore.model.GetBeaconKeyInput;
 import software.amazon.cryptography.keystore.model.GetBeaconKeyOutput;
 import software.amazon.cryptography.keystore.model.GetBranchKeyVersionInput;
 import software.amazon.cryptography.keystore.model.GetBranchKeyVersionOutput;
+import software.amazon.cryptography.keystore.model.GetEncryptedActiveBranchKeyInput;
+import software.amazon.cryptography.keystore.model.GetEncryptedActiveBranchKeyOutput;
+import software.amazon.cryptography.keystore.model.GetEncryptedBeaconKeyInput;
+import software.amazon.cryptography.keystore.model.GetEncryptedBeaconKeyOutput;
+import software.amazon.cryptography.keystore.model.GetEncryptedBranchKeyVersionInput;
+import software.amazon.cryptography.keystore.model.GetEncryptedBranchKeyVersionOutput;
 import software.amazon.cryptography.keystore.model.GetKeyStoreInfoOutput;
+import software.amazon.cryptography.keystore.model.GetTableNameInput;
+import software.amazon.cryptography.keystore.model.GetTableNameOutput;
 import software.amazon.cryptography.keystore.model.KMSConfiguration;
+import software.amazon.cryptography.keystore.model.KeyManagement;
 import software.amazon.cryptography.keystore.model.KeyStoreConfig;
 import software.amazon.cryptography.keystore.model.KeyStoreException;
 import software.amazon.cryptography.keystore.model.MRDiscovery;
 import software.amazon.cryptography.keystore.model.OpaqueError;
+import software.amazon.cryptography.keystore.model.Storage;
 import software.amazon.cryptography.keystore.model.VersionKeyInput;
 import software.amazon.cryptography.keystore.model.VersionKeyOutput;
+import software.amazon.cryptography.keystore.model.WriteNewBranchKeyVersionToKeystoreInput;
+import software.amazon.cryptography.keystore.model.WriteNewBranchKeyVersionToKeystoreOutput;
+import software.amazon.cryptography.keystore.model.WriteNewKeyToStoreInput;
+import software.amazon.cryptography.keystore.model.WriteNewKeyToStoreOutput;
 
 public class ToNative {
 
@@ -96,6 +115,33 @@ public class ToNative {
     }
     OpaqueError.Builder nativeBuilder = OpaqueError.builder();
     nativeBuilder.obj(dafnyValue);
+    return nativeBuilder.build();
+  }
+
+  public static ActiveHierarchicalSymmetricBeacon ActiveHierarchicalSymmetricBeacon(
+    software.amazon.cryptography.keystore.internaldafny.types.ActiveHierarchicalSymmetricBeacon dafnyValue
+  ) {
+    ActiveHierarchicalSymmetricBeacon.Builder nativeBuilder =
+      ActiveHierarchicalSymmetricBeacon.builder();
+    return nativeBuilder.build();
+  }
+
+  public static AwsKms AwsKms(
+    software.amazon.cryptography.keystore.internaldafny.types.AwsKms dafnyValue
+  ) {
+    AwsKms.Builder nativeBuilder = AwsKms.builder();
+    if (dafnyValue.dtor_grantTokens().is_Some()) {
+      nativeBuilder.grantTokens(
+        ToNative.GrantTokenList(dafnyValue.dtor_grantTokens().dtor_value())
+      );
+    }
+    if (dafnyValue.dtor_kmsClient().is_Some()) {
+      nativeBuilder.kmsClient(
+        software.amazon.cryptography.services.kms.internaldafny.ToNative.TrentService(
+          dafnyValue.dtor_kmsClient().dtor_value()
+        )
+      );
+    }
     return nativeBuilder.build();
   }
 
@@ -210,6 +256,57 @@ public class ToNative {
     return nativeBuilder.build();
   }
 
+  public static DynamoDBTable DynamoDBTable(
+    software.amazon.cryptography.keystore.internaldafny.types.DynamoDBTable dafnyValue
+  ) {
+    DynamoDBTable.Builder nativeBuilder = DynamoDBTable.builder();
+    nativeBuilder.ddbTableName(
+      software.amazon.smithy.dafny.conversion.ToNative.Simple.String(
+        dafnyValue.dtor_ddbTableName()
+      )
+    );
+    if (dafnyValue.dtor_ddbClient().is_Some()) {
+      nativeBuilder.ddbClient(
+        software.amazon.cryptography.services.dynamodb.internaldafny.ToNative.DynamoDB_20120810(
+          dafnyValue.dtor_ddbClient().dtor_value()
+        )
+      );
+    }
+    return nativeBuilder.build();
+  }
+
+  public static EncryptedHierarchicalKey EncryptedHierarchicalKey(
+    software.amazon.cryptography.keystore.internaldafny.types.EncryptedHierarchicalKey dafnyValue
+  ) {
+    EncryptedHierarchicalKey.Builder nativeBuilder =
+      EncryptedHierarchicalKey.builder();
+    nativeBuilder.Identifier(
+      software.amazon.smithy.dafny.conversion.ToNative.Simple.String(
+        dafnyValue.dtor_Identifier()
+      )
+    );
+    nativeBuilder.Type(ToNative.BranchKeyType(dafnyValue.dtor_Type()));
+    nativeBuilder.CreateTime(
+      software.amazon.smithy.dafny.conversion.ToNative.Simple.String(
+        dafnyValue.dtor_CreateTime()
+      )
+    );
+    nativeBuilder.KmsArn(
+      software.amazon.smithy.dafny.conversion.ToNative.Simple.String(
+        dafnyValue.dtor_KmsArn()
+      )
+    );
+    nativeBuilder.EncryptionContext(
+      ToNative.EncryptionContextString(dafnyValue.dtor_EncryptionContext())
+    );
+    nativeBuilder.CiphertextBlob(
+      software.amazon.smithy.dafny.conversion.ToNative.Simple.ByteBuffer(
+        dafnyValue.dtor_CiphertextBlob()
+      )
+    );
+    return nativeBuilder.build();
+  }
+
   public static GetActiveBranchKeyInput GetActiveBranchKeyInput(
     software.amazon.cryptography.keystore.internaldafny.types.GetActiveBranchKeyInput dafnyValue
   ) {
@@ -285,6 +382,83 @@ public class ToNative {
     return nativeBuilder.build();
   }
 
+  public static GetEncryptedActiveBranchKeyInput GetEncryptedActiveBranchKeyInput(
+    software.amazon.cryptography.keystore.internaldafny.types.GetEncryptedActiveBranchKeyInput dafnyValue
+  ) {
+    GetEncryptedActiveBranchKeyInput.Builder nativeBuilder =
+      GetEncryptedActiveBranchKeyInput.builder();
+    nativeBuilder.Identifier(
+      software.amazon.smithy.dafny.conversion.ToNative.Simple.String(
+        dafnyValue.dtor_Identifier()
+      )
+    );
+    return nativeBuilder.build();
+  }
+
+  public static GetEncryptedActiveBranchKeyOutput GetEncryptedActiveBranchKeyOutput(
+    software.amazon.cryptography.keystore.internaldafny.types.GetEncryptedActiveBranchKeyOutput dafnyValue
+  ) {
+    GetEncryptedActiveBranchKeyOutput.Builder nativeBuilder =
+      GetEncryptedActiveBranchKeyOutput.builder();
+    nativeBuilder.Item(
+      ToNative.EncryptedHierarchicalKey(dafnyValue.dtor_Item())
+    );
+    return nativeBuilder.build();
+  }
+
+  public static GetEncryptedBeaconKeyInput GetEncryptedBeaconKeyInput(
+    software.amazon.cryptography.keystore.internaldafny.types.GetEncryptedBeaconKeyInput dafnyValue
+  ) {
+    GetEncryptedBeaconKeyInput.Builder nativeBuilder =
+      GetEncryptedBeaconKeyInput.builder();
+    nativeBuilder.Identifier(
+      software.amazon.smithy.dafny.conversion.ToNative.Simple.String(
+        dafnyValue.dtor_Identifier()
+      )
+    );
+    return nativeBuilder.build();
+  }
+
+  public static GetEncryptedBeaconKeyOutput GetEncryptedBeaconKeyOutput(
+    software.amazon.cryptography.keystore.internaldafny.types.GetEncryptedBeaconKeyOutput dafnyValue
+  ) {
+    GetEncryptedBeaconKeyOutput.Builder nativeBuilder =
+      GetEncryptedBeaconKeyOutput.builder();
+    nativeBuilder.Item(
+      ToNative.EncryptedHierarchicalKey(dafnyValue.dtor_Item())
+    );
+    return nativeBuilder.build();
+  }
+
+  public static GetEncryptedBranchKeyVersionInput GetEncryptedBranchKeyVersionInput(
+    software.amazon.cryptography.keystore.internaldafny.types.GetEncryptedBranchKeyVersionInput dafnyValue
+  ) {
+    GetEncryptedBranchKeyVersionInput.Builder nativeBuilder =
+      GetEncryptedBranchKeyVersionInput.builder();
+    nativeBuilder.Identifier(
+      software.amazon.smithy.dafny.conversion.ToNative.Simple.String(
+        dafnyValue.dtor_Identifier()
+      )
+    );
+    nativeBuilder.Version(
+      software.amazon.smithy.dafny.conversion.ToNative.Simple.String(
+        dafnyValue.dtor_Version()
+      )
+    );
+    return nativeBuilder.build();
+  }
+
+  public static GetEncryptedBranchKeyVersionOutput GetEncryptedBranchKeyVersionOutput(
+    software.amazon.cryptography.keystore.internaldafny.types.GetEncryptedBranchKeyVersionOutput dafnyValue
+  ) {
+    GetEncryptedBranchKeyVersionOutput.Builder nativeBuilder =
+      GetEncryptedBranchKeyVersionOutput.builder();
+    nativeBuilder.Item(
+      ToNative.EncryptedHierarchicalKey(dafnyValue.dtor_Item())
+    );
+    return nativeBuilder.build();
+  }
+
   public static GetKeyStoreInfoOutput GetKeyStoreInfoOutput(
     software.amazon.cryptography.keystore.internaldafny.types.GetKeyStoreInfoOutput dafnyValue
   ) {
@@ -314,15 +488,29 @@ public class ToNative {
     return nativeBuilder.build();
   }
 
+  public static GetTableNameInput GetTableNameInput(
+    software.amazon.cryptography.keystore.internaldafny.types.GetTableNameInput dafnyValue
+  ) {
+    GetTableNameInput.Builder nativeBuilder = GetTableNameInput.builder();
+    return nativeBuilder.build();
+  }
+
+  public static GetTableNameOutput GetTableNameOutput(
+    software.amazon.cryptography.keystore.internaldafny.types.GetTableNameOutput dafnyValue
+  ) {
+    GetTableNameOutput.Builder nativeBuilder = GetTableNameOutput.builder();
+    nativeBuilder.Name(
+      software.amazon.smithy.dafny.conversion.ToNative.Simple.DafnyUtf8Bytes(
+        dafnyValue.dtor_Name()
+      )
+    );
+    return nativeBuilder.build();
+  }
+
   public static KeyStoreConfig KeyStoreConfig(
     software.amazon.cryptography.keystore.internaldafny.types.KeyStoreConfig dafnyValue
   ) {
     KeyStoreConfig.Builder nativeBuilder = KeyStoreConfig.builder();
-    nativeBuilder.ddbTableName(
-      software.amazon.smithy.dafny.conversion.ToNative.Simple.String(
-        dafnyValue.dtor_ddbTableName()
-      )
-    );
     nativeBuilder.kmsConfiguration(
       ToNative.KMSConfiguration(dafnyValue.dtor_kmsConfiguration())
     );
@@ -331,6 +519,18 @@ public class ToNative {
         dafnyValue.dtor_logicalKeyStoreName()
       )
     );
+    if (dafnyValue.dtor_keyManagement().is_Some()) {
+      nativeBuilder.keyManagement(
+        ToNative.KeyManagement(dafnyValue.dtor_keyManagement().dtor_value())
+      );
+    }
+    if (dafnyValue.dtor_ddbTableName().is_Some()) {
+      nativeBuilder.ddbTableName(
+        software.amazon.smithy.dafny.conversion.ToNative.Simple.String(
+          dafnyValue.dtor_ddbTableName().dtor_value()
+        )
+      );
+    }
     if (dafnyValue.dtor_id().is_Some()) {
       nativeBuilder.id(
         software.amazon.smithy.dafny.conversion.ToNative.Simple.String(
@@ -341,6 +541,11 @@ public class ToNative {
     if (dafnyValue.dtor_grantTokens().is_Some()) {
       nativeBuilder.grantTokens(
         ToNative.GrantTokenList(dafnyValue.dtor_grantTokens().dtor_value())
+      );
+    }
+    if (dafnyValue.dtor_storage().is_Some()) {
+      nativeBuilder.storage(
+        ToNative.Storage(dafnyValue.dtor_storage().dtor_value())
       );
     }
     if (dafnyValue.dtor_ddbClient().is_Some()) {
@@ -391,6 +596,94 @@ public class ToNative {
     return nativeBuilder.build();
   }
 
+  public static WriteNewBranchKeyVersionToKeystoreInput WriteNewBranchKeyVersionToKeystoreInput(
+    software.amazon.cryptography.keystore.internaldafny.types.WriteNewBranchKeyVersionToKeystoreInput dafnyValue
+  ) {
+    WriteNewBranchKeyVersionToKeystoreInput.Builder nativeBuilder =
+      WriteNewBranchKeyVersionToKeystoreInput.builder();
+    nativeBuilder.Active(
+      ToNative.EncryptedHierarchicalKey(dafnyValue.dtor_Active())
+    );
+    nativeBuilder.Version(
+      ToNative.EncryptedHierarchicalKey(dafnyValue.dtor_Version())
+    );
+    nativeBuilder.oldActive(
+      ToNative.EncryptedHierarchicalKey(dafnyValue.dtor_oldActive())
+    );
+    return nativeBuilder.build();
+  }
+
+  public static WriteNewBranchKeyVersionToKeystoreOutput WriteNewBranchKeyVersionToKeystoreOutput(
+    software.amazon.cryptography.keystore.internaldafny.types.WriteNewBranchKeyVersionToKeystoreOutput dafnyValue
+  ) {
+    WriteNewBranchKeyVersionToKeystoreOutput.Builder nativeBuilder =
+      WriteNewBranchKeyVersionToKeystoreOutput.builder();
+    return nativeBuilder.build();
+  }
+
+  public static WriteNewKeyToStoreInput WriteNewKeyToStoreInput(
+    software.amazon.cryptography.keystore.internaldafny.types.WriteNewKeyToStoreInput dafnyValue
+  ) {
+    WriteNewKeyToStoreInput.Builder nativeBuilder =
+      WriteNewKeyToStoreInput.builder();
+    nativeBuilder.Active(
+      ToNative.EncryptedHierarchicalKey(dafnyValue.dtor_Active())
+    );
+    nativeBuilder.Version(
+      ToNative.EncryptedHierarchicalKey(dafnyValue.dtor_Version())
+    );
+    nativeBuilder.Beacon(
+      ToNative.EncryptedHierarchicalKey(dafnyValue.dtor_Beacon())
+    );
+    return nativeBuilder.build();
+  }
+
+  public static WriteNewKeyToStoreOutput WriteNewKeyToStoreOutput(
+    software.amazon.cryptography.keystore.internaldafny.types.WriteNewKeyToStoreOutput dafnyValue
+  ) {
+    WriteNewKeyToStoreOutput.Builder nativeBuilder =
+      WriteNewKeyToStoreOutput.builder();
+    return nativeBuilder.build();
+  }
+
+  public static BranchKeyType BranchKeyType(
+    software.amazon.cryptography.keystore.internaldafny.types.BranchKeyType dafnyValue
+  ) {
+    BranchKeyType.Builder nativeBuilder = BranchKeyType.builder();
+    if (dafnyValue.is_ActiveHierarchicalSymmetricVersion()) {
+      nativeBuilder.ActiveHierarchicalSymmetricVersion(
+        software.amazon.smithy.dafny.conversion.ToNative.Simple.String(
+          dafnyValue.dtor_ActiveHierarchicalSymmetricVersion()
+        )
+      );
+    }
+    if (dafnyValue.is_HierarchicalSymmetricVersion()) {
+      nativeBuilder.HierarchicalSymmetricVersion(
+        software.amazon.smithy.dafny.conversion.ToNative.Simple.String(
+          dafnyValue.dtor_HierarchicalSymmetricVersion()
+        )
+      );
+    }
+    if (dafnyValue.is_ActiveHierarchicalSymmetricBeacon()) {
+      nativeBuilder.ActiveHierarchicalSymmetricBeacon(
+        ToNative.ActiveHierarchicalSymmetricBeacon(
+          dafnyValue.dtor_ActiveHierarchicalSymmetricBeacon()
+        )
+      );
+    }
+    return nativeBuilder.build();
+  }
+
+  public static KeyManagement KeyManagement(
+    software.amazon.cryptography.keystore.internaldafny.types.KeyManagement dafnyValue
+  ) {
+    KeyManagement.Builder nativeBuilder = KeyManagement.builder();
+    if (dafnyValue.is_kms()) {
+      nativeBuilder.kms(ToNative.AwsKms(dafnyValue.dtor_kms()));
+    }
+    return nativeBuilder.build();
+  }
+
   public static KMSConfiguration KMSConfiguration(
     software.amazon.cryptography.keystore.internaldafny.types.KMSConfiguration dafnyValue
   ) {
@@ -420,6 +713,21 @@ public class ToNative {
     return nativeBuilder.build();
   }
 
+  public static Storage Storage(
+    software.amazon.cryptography.keystore.internaldafny.types.Storage dafnyValue
+  ) {
+    Storage.Builder nativeBuilder = Storage.builder();
+    if (dafnyValue.is_ddb()) {
+      nativeBuilder.ddb(ToNative.DynamoDBTable(dafnyValue.dtor_ddb()));
+    }
+    if (dafnyValue.is_custom()) {
+      nativeBuilder.custom(
+        ToNative.EncryptedKeyStore(dafnyValue.dtor_custom())
+      );
+    }
+    return nativeBuilder.build();
+  }
+
   public static List<String> GrantTokenList(
     DafnySequence<? extends DafnySequence<? extends Character>> dafnyValue
   ) {
@@ -442,6 +750,19 @@ public class ToNative {
     );
   }
 
+  public static Map<String, String> EncryptionContextString(
+    DafnyMap<
+      ? extends DafnySequence<? extends Character>,
+      ? extends DafnySequence<? extends Character>
+    > dafnyValue
+  ) {
+    return software.amazon.smithy.dafny.conversion.ToNative.Aggregate.GenericToMap(
+      dafnyValue,
+      software.amazon.smithy.dafny.conversion.ToNative.Simple::String,
+      software.amazon.smithy.dafny.conversion.ToNative.Simple::String
+    );
+  }
+
   public static Map<String, ByteBuffer> HmacKeyMap(
     DafnyMap<
       ? extends DafnySequence<? extends Character>,
@@ -453,6 +774,15 @@ public class ToNative {
       software.amazon.smithy.dafny.conversion.ToNative.Simple::String,
       software.amazon.smithy.dafny.conversion.ToNative.Simple::ByteBuffer
     );
+  }
+
+  public static IEncryptedKeyStore EncryptedKeyStore(
+    software.amazon.cryptography.keystore.internaldafny.types.IEncryptedKeyStore dafnyValue
+  ) {
+    if (dafnyValue instanceof EncryptedKeyStore.NativeWrapper) {
+      return ((EncryptedKeyStore.NativeWrapper) dafnyValue)._impl;
+    }
+    return EncryptedKeyStore.wrap(dafnyValue);
   }
 
   public static KeyStore KeyStore(IKeyStoreClient dafnyValue) {
