AwsCryptographicMaterialProviders/runtimes/java/src/main/smithy-generated/software/amazon/cryptography/keystore/model/GetTableNameOutput.java
@@ -1,0 +1,64 @@
+// Copyright Amazon.com Inc. or its affiliates. All Rights Reserved.
+// SPDX-License-Identifier: Apache-2.0
+// Do not modify this file. This file is machine generated, and any changes to it will be overwritten.
+package software.amazon.cryptography.keystore.model;
+
+import java.util.Objects;
+
+public class GetTableNameOutput {
+
+  private final String Name;
+
+  protected GetTableNameOutput(BuilderImpl builder) {
+    this.Name = builder.Name();
+  }
+
+  public String Name() {
+    return this.Name;
+  }
+
+  public Builder toBuilder() {
+    return new BuilderImpl(this);
+  }
+
+  public static Builder builder() {
+    return new BuilderImpl();
+  }
+
+  public interface Builder {
+    Builder Name(String Name);
+
+    String Name();
+
+    GetTableNameOutput build();
+  }
+
+  static class BuilderImpl implements Builder {
+
+    protected String Name;
+
+    protected BuilderImpl() {}
+
+    protected BuilderImpl(GetTableNameOutput model) {
+      this.Name = model.Name();
+    }
+
+    public Builder Name(String Name) {
+      this.Name = Name;
+      return this;
+    }
+
+    public String Name() {
+      return this.Name;
+    }
+
+    public GetTableNameOutput build() {
+      if (Objects.isNull(this.Name())) {
+        throw new IllegalArgumentException(
+          "Missing value for required field `Name`"
+        );
+      }
+      return new GetTableNameOutput(this);
+    }
+  }
+}
