AwsCryptographicMaterialProviders/runtimes/net/Generated/AwsCryptographyKeyStore/IEncryptedKeyStore.cs
@@ -1,0 +1,17 @@
+// Copyright Amazon.com Inc. or its affiliates. All Rights Reserved.
+// SPDX-License-Identifier: Apache-2.0
+// Do not modify this file. This file is machine generated, and any changes to it will be overwritten.
+using System;
+using AWS.Cryptography.KeyStore;
+namespace AWS.Cryptography.KeyStore
+{
+  public interface IEncryptedKeyStore
+  {
+    AWS.Cryptography.KeyStore.WriteNewKeyToStoreOutput WriteNewKeyToStore(AWS.Cryptography.KeyStore.WriteNewKeyToStoreInput input);
+    AWS.Cryptography.KeyStore.WriteNewBranchKeyVersionToKeystoreOutput WriteNewBranchKeyVersionToKeystore(AWS.Cryptography.KeyStore.WriteNewBranchKeyVersionToKeystoreInput input);
+    AWS.Cryptography.KeyStore.GetEncryptedActiveBranchKeyOutput GetEncryptedActiveBranchKey(AWS.Cryptography.KeyStore.GetEncryptedActiveBranchKeyInput input);
+    AWS.Cryptography.KeyStore.GetEncryptedBranchKeyVersionOutput GetEncryptedBranchKeyVersion(AWS.Cryptography.KeyStore.GetEncryptedBranchKeyVersionInput input);
+    AWS.Cryptography.KeyStore.GetEncryptedBeaconKeyOutput GetEncryptedBeaconKey(AWS.Cryptography.KeyStore.GetEncryptedBeaconKeyInput input);
+    AWS.Cryptography.KeyStore.GetTableNameOutput GetTableName(AWS.Cryptography.KeyStore.GetTableNameInput input);
+  }
+}
