AwsCryptographicMaterialProviders/dafny/AwsCryptographyKeyStore/Model/Storage.smithy
@@ -1,0 +1,203 @@
+// Copyright Amazon.com Inc. or its affiliates. All Rights Reserved.
+// SPDX-License-Identifier: Apache-2.0
+namespace aws.cryptography.keyStore
+
+
+//= aws-encryption-sdk-specification/framework/key-store/encrypted-key-store.md#type
+//= type=implication
+//# A union that MUST hold the following three options
+//#
+//#- ActiveHierarchicalSymmetricVersion [HierarchicalSymmetricVersion](#hierarchicalsymmetricversion)
+//#- HierarchicalSymmetricVersion [HierarchicalSymmetricVersion](#hierarchicalsymmetricversion)
+//#- ActiveHierarchicalSymmetricBeacon
+union BranchKeyType {
+  ActiveHierarchicalSymmetricVersion: String,
+  //= aws-encryption-sdk-specification/framework/key-store/encrypted-key-store.md#hierarchicalsymmetricversion
+  //= type=implication
+  //# A structure that MUST have one member,
+  //# the UTF8 Encoded value of the version of the branch key.
+  HierarchicalSymmetricVersion: String,
+  ActiveHierarchicalSymmetricBeacon: ActiveHierarchicalSymmetricBeacon
+}
+
+structure ActiveHierarchicalSymmetricBeacon {}
+
+
+//= aws-encryption-sdk-specification/framework/key-store/encrypted-key-store.md#encryptedhierarchicalkey
+//= type=implication
+//# This structure MUST include all of the following fields:
+//#
+//#- [BranchKeyId](./structures.md#branch-key-id)
+//#- [Type](#type)
+//#- CreateTime: Timestamp in ISO 8601 format in UTC, to microsecond precision.
+//#- KmsArn: The AWS KMS Key ARN used to protect the CiphertextBlob value.
+//#- [EncryptionContext](./structures.md#encryption-context-3)
+//#- CiphertextBlob: The encrypted binary for the hierarchical key.
+structure EncryptedHierarchicalKey {
+  @required
+  Identifier: String,
+
+  @required
+  Type: BranchKeyType,
+
+  @required
+  CreateTime: String,
+
+  @required
+  KmsArn: String,
+
+  @required
+  EncryptionContext: EncryptionContextString,
+
+  @required
+  CiphertextBlob: Blob,
+}
+
+map EncryptionContextString {
+  key: String,
+  value: String,
+}
+
+@aws.polymorph#extendable
+resource EncryptedKeyStore {
+
+//= aws-encryption-sdk-specification/framework/key-store/encrypted-key-store.md#interface
+//= type=implication
+//# The EncryptedKeyStore MUST support the following operations:
+//#
+//#- [WriteNewKeyToStore](#writenewkeytostore)
+//#- [WriteNewBranchKeyVersionToKeystore](#writenewbranchkeyversiontokeystore)
+//#- [GetEncryptedActiveBranchKey](#getencryptedactivebranchkey)
+//#- [GetEncryptedBranchKeyVersion](#getencryptedbranchkeyversion)
+//#- [GetEncryptedBeaconKey](#getencryptedbeaconkey)
+//#- [GetTableName](#gettablename)
+  operations: [
+    WriteNewKeyToStore,
+    WriteNewBranchKeyVersionToKeystore,
+    GetEncryptedActiveBranchKey,
+    GetEncryptedBranchKeyVersion,
+    GetEncryptedBeaconKey,
+    GetTableName,
+  ]
+}
+
+@aws.polymorph#reference(resource: EncryptedKeyStore)
+structure EncryptedKeyStoreReference {}
+
+operation WriteNewKeyToStore {
+  input: WriteNewKeyToStoreInput,
+  output: WriteNewKeyToStoreOutput,
+}
+operation WriteNewBranchKeyVersionToKeystore {
+  input: WriteNewBranchKeyVersionToKeystoreInput,
+  output: WriteNewBranchKeyVersionToKeystoreOutput,
+}
+operation GetEncryptedActiveBranchKey {
+  input: GetEncryptedActiveBranchKeyInput,
+  output: GetEncryptedActiveBranchKeyOutput,
+}
+operation GetEncryptedBranchKeyVersion {
+  input: GetEncryptedBranchKeyVersionInput,
+  output: GetEncryptedBranchKeyVersionOutput,
+}
+operation GetEncryptedBeaconKey {
+  input: GetEncryptedBeaconKeyInput,
+  output: GetEncryptedBeaconKeyOutput,
+}
+operation GetTableName {
+  input: GetTableNameInput,
+  output: GetTableNameOutput,
+}
+
+//= aws-encryption-sdk-specification/framework/key-store/encrypted-key-store.md#writenewkeytostore
+//= type=implication
+//# The WriteNewKeyToStore caller MUST provide:
+//#
+//#- An [EncryptedHierarchicalKey](#encryptedhierarchicalkey) with a [type](#type) of ActiveHierarchicalSymmetricVersion
+//#- An [EncryptedHierarchicalKey](#encryptedhierarchicalkey) with a [type](#type) of HierarchicalSymmetricVersion
+//#- An [EncryptedHierarchicalKey](#encryptedhierarchicalkey) with a [type](#type) of ActiveHierarchicalSymmetricBeacon
+structure WriteNewKeyToStoreInput {
+  @required
+  Active: EncryptedHierarchicalKey,
+  @required
+  Version: EncryptedHierarchicalKey,
+  @required
+  Beacon: EncryptedHierarchicalKey,
+}
+//= aws-encryption-sdk-specification/framework/key-store/dynamodb-encrypted-key-store.md#writenewkeytostore
+//= type=implication
+//# If DDB TransactWriteItems is successful, this operation MUST return a successful response containing no additional data.
+structure WriteNewKeyToStoreOutput {}
+//= aws-encryption-sdk-specification/framework/key-store/encrypted-key-store.md#writenewbranchkeyversiontokeystore
+//= type=implication
+//# The WriteNewBranchKeyVersionToKeystore caller MUST provide:
+//#
+//#- An [EncryptedHierarchicalKey](#encryptedhierarchicalkey) with a [type](#type) of ActiveHierarchicalSymmetricVersion
+//#- An [EncryptedHierarchicalKey](#encryptedhierarchicalkey) with a [type](#type) of HierarchicalSymmetricVersion
+structure WriteNewBranchKeyVersionToKeystoreInput {
+  @required
+  Active: EncryptedHierarchicalKey,
+  @required
+  Version: EncryptedHierarchicalKey,
+  @required
+  oldActive: EncryptedHierarchicalKey
+}
+structure WriteNewBranchKeyVersionToKeystoreOutput {}
+structure GetEncryptedActiveBranchKeyInput {
+
+  //= aws-encryption-sdk-specification/framework/key-store/encrypted-key-store.md#getencryptedactivebranchkey
+  //= type=implication
+  //# The GetEncryptedActiveBranchKey caller MUST provide the same inputs as the [GetActiveBranchKey](../branch-key-store.md#getactivebranchkey) operation.
+
+  @required
+  Identifier: String,
+}
+//= aws-encryption-sdk-specification/framework/key-store/encrypted-key-store.md#getencryptedactivebranchkey
+//= type=implication
+//# It MUST return an [EncryptedHierarchicalKey](#encryptedhierarchicalkey).
+structure GetEncryptedActiveBranchKeyOutput {
+  @required
+  Item: EncryptedHierarchicalKey,
+}
+structure GetEncryptedBranchKeyVersionInput {
+
+  //= aws-encryption-sdk-specification/framework/key-store/encrypted-key-store.md#getencryptedbranchkeyversion
+  //= type=implication
+  //# The GetEncryptedBranchKeyVersion caller MUST provide the same inputs as the [GetBranchKeyVersion](../branch-key-store.md#getbranchkeyversion) operation.
+
+  @required
+  Identifier: String,
+  @required
+  Version: String,
+}
+//= aws-encryption-sdk-specification/framework/key-store/encrypted-key-store.md#getencryptedbranchkeyversion
+//= type=implication
+//# It MUST return an [EncryptedHierarchicalKey](#encryptedhierarchicalkey).
+structure GetEncryptedBranchKeyVersionOutput {
+  @required
+  Item: EncryptedHierarchicalKey,
+}
+structure GetEncryptedBeaconKeyInput {
+
+  //= aws-encryption-sdk-specification/framework/key-store/encrypted-key-store.md#getencryptedbeaconkey
+  //= type=implication
+  //# The GetEncryptedBeaconKey caller MUST provide the same inputs as the [GetBeaconKey](../branch-key-store.md#getbeaconkey) operation.
+
+  @required
+  Identifier: String,
+}
+//= aws-encryption-sdk-specification/framework/key-store/encrypted-key-store.md#getencryptedbeaconkey
+//= type=implication
+//# It MUST return an [EncryptedHierarchicalKey](#encryptedhierarchicalkey).
+structure GetEncryptedBeaconKeyOutput {
+  @required
+  Item: EncryptedHierarchicalKey,
+}
+structure GetTableNameInput {}
+//= aws-encryption-sdk-specification/framework/key-store/encrypted-key-store.md#gettablename
+//= type=implication
+//# It MUST return the physical table name.
+structure GetTableNameOutput {
+  @required
+  Name: Utf8Bytes,
+}
